\section{Proof splitting matrix}
\label{sec:proofsplittingmatrix}

\begin{equation*}
    \sum _{i=0}^{n-j} \binom{n-j}{i}x^{i+j}y^j(1-x)^{n-j-i}(1-y)^i 
\end{equation*}
\begin{equation*}
    =(xy)^j\sum _{i=0}^{n-j} \binom{n-j}{i}x^i(1-x)^{n-j-i}(1-y)^i 
\end{equation*}

We use this identity to further expand
\begin{equation*}
    (1-x)^n =
    \sum_{i = 0}^{n} {n \choose i} (-1)^{i}(x)^{i}
\end{equation*}

And get this
\begin{equation*}
    =(xy)^j\sum _{i=0}^{n-j} \binom{n-j}{i}x^i
    (\sum_{k = 0}^{n-j-i} {n-j-i \choose k} (-1)^{k}(x)^{k})
    (\sum_{k = 0}^{i} {i \choose k} (-1)^{k}(y)^{k})
\end{equation*}

\begin{equation*}
    =(xy)^j\sum _{i=0}^{n-j}x^i
    (\sum_{k = 0}^{n-j-i} \binom{n-j}{i}{n-j-i \choose k} (-1)^{k}(x)^{k})
    (\sum_{k = 0}^{i} \binom{n-j}{i}{i \choose k} (-1)^{k}(y)^{k})
\end{equation*}